<?xml version="1.0"?>
<rdf:RDF xmlns="http://w3id.org/abdn/policy/pope#"
     xml:base="http://w3id.org/abdn/policy/pope"
     xmlns:rdf="http://www.w3.org/1999/02/22-rdf-syntax-ns#"
     xmlns:terms="http://purl.org/dc/terms/"
     xmlns:owl="http://www.w3.org/2002/07/owl#"
     xmlns:xml="http://www.w3.org/XML/1998/namespace"
     xmlns:xsd="http://www.w3.org/2001/XMLSchema#"
     xmlns:skos="http://www.w3.org/2004/02/skos/core#"
     xmlns:rdfs="http://www.w3.org/2000/01/rdf-schema#"
     xmlns:prov="http://www.w3.org/ns/prov#">
    <owl:Ontology rdf:about="http://w3id.org/abdn/policy/pope">
        <owl:imports rdf:resource="http://www.w3.org/ns/prov-o-20130430"/>
        <owl:imports rdf:resource="http://www.w3.org/2004/02/skos/core"/>
        <terms:creator rdf:datatype="http://www.w3.org/2001/XMLSchema#string">Chenghua Lin</terms:creator>
        <terms:creator rdf:datatype="http://www.w3.org/2001/XMLSchema#string">Peter Edwards</terms:creator>
        <terms:description rdf:datatype="http://www.w3.org/2001/XMLSchema#string">The PoPE Provenance Vocabulary defines a set of concepts and terms (the vocabulary)  for describing the use of social media data as evidence in policy-making.</terms:description>
        <rdfs:label rdf:datatype="http://www.w3.org/2001/XMLSchema#string">PoPE Version 1.0</rdfs:label>
        <terms:license rdf:datatype="http://www.w3.org/2001/XMLSchema#string">https://creativecommons.org/licenses/by/4.0/</terms:license>
        <terms:creator rdf:datatype="http://www.w3.org/2001/XMLSchema#string">David Corsar</terms:creator>
        <owl:versionInfo rdf:datatype="http://www.w3.org/2001/XMLSchema#string">1.0</owl:versionInfo>
        <terms:creator rdf:datatype="http://www.w3.org/2001/XMLSchema#string">Milan Markovic</terms:creator>
    </owl:Ontology>
    


    <!-- 
    ///////////////////////////////////////////////////////////////////////////////////////
    //
    // Object Properties
    //
    ///////////////////////////////////////////////////////////////////////////////////////
     -->

    


    <!-- http://w3id.org/abdn/policy/pope#appliesTo -->

    <owl:ObjectProperty rdf:about="http://w3id.org/abdn/policy/pope#appliesTo">
        <rdfs:subPropertyOf rdf:resource="http://www.w3.org/2004/02/skos/core#related"/>
        <rdfs:comment xml:lang="en">A appliesTo B denotes that the instance A describes some concept relevant to B and where A is not part of B. For example, a license applied to a collection of data items.</rdfs:comment>
        <rdfs:label xml:lang="en">appliesTo</rdfs:label>
    </owl:ObjectProperty>
    


    <!-- http://w3id.org/abdn/policy/pope#describedAs -->

    <owl:ObjectProperty rdf:about="http://w3id.org/abdn/policy/pope#describedAs">
        <rdfs:subPropertyOf rdf:resource="http://www.w3.org/2004/02/skos/core#narrower"/>
    </owl:ObjectProperty>
    


    <!-- http://w3id.org/abdn/policy/pope#doesNotMatch -->

    <owl:ObjectProperty rdf:about="http://w3id.org/abdn/policy/pope#doesNotMatch">
        <rdfs:subPropertyOf rdf:resource="http://www.w3.org/2004/02/skos/core#related"/>
        <rdfs:comment xml:lang="en">A matches B denotes that the expression described by the instance A cannot be matched on some value described by the instance B. For example, if A describes a regular expression, it cannnot be matched on a piece of text described by B.</rdfs:comment>
        <rdfs:label xml:lang="en">doesNotMatch</rdfs:label>
    </owl:ObjectProperty>
    


    <!-- http://w3id.org/abdn/policy/pope#includedIn -->

    <owl:ObjectProperty rdf:about="http://w3id.org/abdn/policy/pope#includedIn">
        <rdfs:subPropertyOf rdf:resource="http://www.w3.org/2004/02/skos/core#related"/>
        <owl:inverseOf rdf:resource="http://w3id.org/abdn/policy/pope#includes"/>
        <rdfs:comment xml:lang="en">A includedIn B denotes that the instance A describes a part of instance B. For example, if B is a dataset item, A can represent a portion of that item, for example, a body of a post contianed within B.</rdfs:comment>
        <rdfs:label xml:lang="en">includedIn</rdfs:label>
    </owl:ObjectProperty>
    


    <!-- http://w3id.org/abdn/policy/pope#includes -->

    <owl:ObjectProperty rdf:about="http://w3id.org/abdn/policy/pope#includes">
        <rdfs:subPropertyOf rdf:resource="http://www.w3.org/2004/02/skos/core#related"/>
        <rdfs:comment xml:lang="en">A includes B denotes that the instance A describes a concept that includes B. For example, if A is describing an area covering the UK, B can describe the city of London.</rdfs:comment>
        <rdfs:label xml:lang="en">includes</rdfs:label>
    </owl:ObjectProperty>
    


    <!-- http://w3id.org/abdn/policy/pope#isEqualTo -->

    <owl:ObjectProperty rdf:about="http://w3id.org/abdn/policy/pope#isEqualTo">
        <rdfs:subPropertyOf rdf:resource="http://www.w3.org/2004/02/skos/core#related"/>
        <rdf:type rdf:resource="http://www.w3.org/2002/07/owl#SymmetricProperty"/>
        <rdfs:comment xml:lang="en">A isEqualTo B denotes that the value represented by instance A is equal to the value represented by instance B, however, A and B are not the same. For exampel, a red glass of water can be equal to a blue glass of water of the same size.</rdfs:comment>
        <rdfs:label xml:lang="en">isEqualTo</rdfs:label>
    </owl:ObjectProperty>
    


    <!-- http://w3id.org/abdn/policy/pope#lessThan -->

    <owl:ObjectProperty rdf:about="http://w3id.org/abdn/policy/pope#lessThan">
        <rdfs:subPropertyOf rdf:resource="http://www.w3.org/2004/02/skos/core#related"/>
        <owl:inverseOf rdf:resource="http://w3id.org/abdn/policy/pope#moreThan"/>
        <rdfs:comment xml:lang="en">A lessThan B denotes that the quantity represented by instance A is lower than the quantity represented by instance B.</rdfs:comment>
        <rdfs:label xml:lang="en">lessThan</rdfs:label>
    </owl:ObjectProperty>
    


    <!-- http://w3id.org/abdn/policy/pope#lessThanOrEqualTo -->

    <owl:ObjectProperty rdf:about="http://w3id.org/abdn/policy/pope#lessThanOrEqualTo">
        <rdfs:subPropertyOf rdf:resource="http://www.w3.org/2004/02/skos/core#related"/>
        <owl:inverseOf rdf:resource="http://w3id.org/abdn/policy/pope#moreThanOrEqualTo"/>
        <rdfs:comment xml:lang="en">A lessThanOrEqualTo B denotes that the quantity represented by instance A is lower or equal to the quantity represented by instance B.</rdfs:comment>
        <rdfs:label xml:lang="en">lessThanOrEqualTo</rdfs:label>
    </owl:ObjectProperty>
    


    <!-- http://w3id.org/abdn/policy/pope#lhs -->

    <owl:ObjectProperty rdf:about="http://w3id.org/abdn/policy/pope#lhs">
        <rdfs:subPropertyOf rdf:resource="http://www.w3.org/2004/02/skos/core#related"/>
        <rdf:type rdf:resource="http://www.w3.org/2002/07/owl#FunctionalProperty"/>
        <rdfs:domain>
            <owl:Class>
                <owl:unionOf rdf:parseType="Collection">
                    <rdf:Description rdf:about="http://w3id.org/abdn/policy/pope#AND_Node"/>
                    <rdf:Description rdf:about="http://w3id.org/abdn/policy/pope#OR_Node"/>
                    <rdf:Description rdf:about="http://w3id.org/abdn/policy/pope#XOR_Node"/>
                </owl:unionOf>
            </owl:Class>
        </rdfs:domain>
        <rdfs:range>
            <owl:Class>
                <owl:unionOf rdf:parseType="Collection">
                    <rdf:Description rdf:about="http://w3id.org/abdn/policy/pope#AND_Node"/>
                    <rdf:Description rdf:about="http://w3id.org/abdn/policy/pope#LeafNode"/>
                    <rdf:Description rdf:about="http://w3id.org/abdn/policy/pope#OR_Node"/>
                    <rdf:Description rdf:about="http://w3id.org/abdn/policy/pope#XOR_Node"/>
                </owl:unionOf>
            </owl:Class>
        </rdfs:range>
        <rdfs:comment xml:lang="en">A property linking a parent node of a binary tree to its left hand side child.</rdfs:comment>
        <rdfs:label xml:lang="en">lhs</rdfs:label>
    </owl:ObjectProperty>
    


    <!-- http://w3id.org/abdn/policy/pope#matches -->

    <owl:ObjectProperty rdf:about="http://w3id.org/abdn/policy/pope#matches">
        <rdfs:subPropertyOf rdf:resource="http://www.w3.org/2004/02/skos/core#related"/>
        <rdfs:comment xml:lang="en">A matches B denotes that the expression described by the instance A can be matched on some value described by the instance B. For example, if A describes a regular expression, it can be matched on a piece of text described by B.</rdfs:comment>
        <rdfs:label xml:lang="en">matches</rdfs:label>
    </owl:ObjectProperty>
    


    <!-- http://w3id.org/abdn/policy/pope#moreThan -->

    <owl:ObjectProperty rdf:about="http://w3id.org/abdn/policy/pope#moreThan">
        <rdfs:subPropertyOf rdf:resource="http://www.w3.org/2004/02/skos/core#related"/>
        <rdfs:comment xml:lang="en">A moreThan B denotes that the quantity represented by instance A is greater than the quantity represented by instance B.</rdfs:comment>
        <rdfs:label xml:lang="en">moreThan</rdfs:label>
    </owl:ObjectProperty>
    


    <!-- http://w3id.org/abdn/policy/pope#moreThanOrEqualTo -->

    <owl:ObjectProperty rdf:about="http://w3id.org/abdn/policy/pope#moreThanOrEqualTo">
        <rdfs:subPropertyOf rdf:resource="http://www.w3.org/2004/02/skos/core#related"/>
        <rdfs:comment xml:lang="en">A moreThanOrEqualTo B denotes that the quantity represented by instance A is greater or equal to the quantity represented by instance B.</rdfs:comment>
        <rdfs:label xml:lang="en">moreThanOrEqualTo</rdfs:label>
    </owl:ObjectProperty>
    


    <!-- http://w3id.org/abdn/policy/pope#notIncludedIn -->

    <owl:ObjectProperty rdf:about="http://w3id.org/abdn/policy/pope#notIncludedIn">
        <rdfs:subPropertyOf rdf:resource="http://www.w3.org/2004/02/skos/core#related"/>
        <rdfs:comment xml:lang="en">A notIncludedIn B denotes that the instance A does not describe any part of instance B. For example, if B represents a piece of text, A can represent a keyword that is not present in B.</rdfs:comment>
        <rdfs:label xml:lang="en">notIncludedIn</rdfs:label>
    </owl:ObjectProperty>
    


    <!-- http://w3id.org/abdn/policy/pope#parameter -->

    <owl:ObjectProperty rdf:about="http://w3id.org/abdn/policy/pope#parameter">
        <rdfs:subPropertyOf rdf:resource="http://www.w3.org/2004/02/skos/core#related"/>
        <rdfs:domain rdf:resource="http://w3id.org/abdn/policy/pope#LeafNode"/>
        <rdfs:range rdf:resource="http://www.w3.org/ns/prov#Entity"/>
        <rdfs:comment xml:lang="en">A property for linking pope:LeafNode to a prov:Entity typically associated with a role of pope:Parameter.</rdfs:comment>
        <rdfs:label xml:lang="en">parameter</rdfs:label>
    </owl:ObjectProperty>
    


    <!-- http://w3id.org/abdn/policy/pope#rhs -->

    <owl:ObjectProperty rdf:about="http://w3id.org/abdn/policy/pope#rhs">
        <rdfs:subPropertyOf rdf:resource="http://www.w3.org/2004/02/skos/core#related"/>
        <rdf:type rdf:resource="http://www.w3.org/2002/07/owl#FunctionalProperty"/>
        <rdfs:domain>
            <owl:Class>
                <owl:unionOf rdf:parseType="Collection">
                    <rdf:Description rdf:about="http://w3id.org/abdn/policy/pope#AND_Node"/>
                    <rdf:Description rdf:about="http://w3id.org/abdn/policy/pope#OR_Node"/>
                    <rdf:Description rdf:about="http://w3id.org/abdn/policy/pope#XOR_Node"/>
                </owl:unionOf>
            </owl:Class>
        </rdfs:domain>
        <rdfs:range>
            <owl:Class>
                <owl:unionOf rdf:parseType="Collection">
                    <rdf:Description rdf:about="http://w3id.org/abdn/policy/pope#AND_Node"/>
                    <rdf:Description rdf:about="http://w3id.org/abdn/policy/pope#LeafNode"/>
                    <rdf:Description rdf:about="http://w3id.org/abdn/policy/pope#OR_Node"/>
                    <rdf:Description rdf:about="http://w3id.org/abdn/policy/pope#XOR_Node"/>
                </owl:unionOf>
            </owl:Class>
        </rdfs:range>
        <rdfs:comment xml:lang="en">A property linking a parent node of a binary tree to its right hand side child.</rdfs:comment>
        <rdfs:label xml:lang="en">rhs</rdfs:label>
    </owl:ObjectProperty>
    


    <!-- 
    ///////////////////////////////////////////////////////////////////////////////////////
    //
    // Classes
    //
    ///////////////////////////////////////////////////////////////////////////////////////
     -->

    


    <!-- http://w3id.org/abdn/policy/pope#AND_Node -->

    <owl:Class rdf:about="http://w3id.org/abdn/policy/pope#AND_Node">
        <rdfs:subClassOf rdf:resource="http://www.w3.org/2004/02/skos/core#Concept"/>
        <owl:disjointWith rdf:resource="http://w3id.org/abdn/policy/pope#LeafNode"/>
        <owl:disjointWith rdf:resource="http://w3id.org/abdn/policy/pope#OR_Node"/>
        <owl:disjointWith rdf:resource="http://w3id.org/abdn/policy/pope#XOR_Node"/>
        <rdfs:comment xml:lang="en">A concept describing an inner node of a binary tree structure. The node represents the logical operator AND in a binary tree description of pope:Constraint. If A is an XOR_Node and B and C are children of A then test on conditions specified by B AND C equals true.</rdfs:comment>
        <rdfs:label xml:lang="en">AND Node</rdfs:label>
    </owl:Class>
    


    <!-- http://w3id.org/abdn/policy/pope#ActivityPlan -->

    <owl:Class rdf:about="http://w3id.org/abdn/policy/pope#ActivityPlan">
        <rdfs:subClassOf rdf:resource="http://www.w3.org/ns/prov#Plan"/>
        <rdfs:comment xml:lang="en">ActivityPlans describe the type of plan followed by an agent to guide their activity in relation to, for example, collection of data, processing of data before analysis, or analysis of the data.  It is not the intent of ActivityPlan to provide a breakdown of the steps or actions that are involved in the plan; this type of information can, if desired, be represented with alternative plan representations.</rdfs:comment>
        <rdfs:label xml:lang="en">Activity Plan</rdfs:label>
    </owl:Class>
    


    <!-- http://w3id.org/abdn/policy/pope#Constraint -->

    <owl:Class rdf:about="http://w3id.org/abdn/policy/pope#Constraint">
        <rdfs:subClassOf rdf:resource="http://www.w3.org/ns/prov#Role"/>
        <rdfs:comment xml:lang="en">A kind of role describing that the associated prov:Entity denoted some condition/state of the world further described by enties associated with role pope:Parameter. It can be further described with pope:describedAs property linking to a  skos:Concept. For example, a binary tree using pope:AND_Node, pope:OR_Node, pope:XOR_Node and pope:LeafNode can be used to represent logical groupings of one or more of activity parameters.</rdfs:comment>
        <rdfs:label xml:lang="en">Constraint</rdfs:label>
    </owl:Class>
    


    <!-- http://w3id.org/abdn/policy/pope#DataAnalysis -->

    <owl:Class rdf:about="http://w3id.org/abdn/policy/pope#DataAnalysis">
        <rdfs:subClassOf rdf:resource="http://w3id.org/abdn/policy/pope#ActivityPlan"/>
        <rdfs:comment xml:lang="en">A kind of  activity plan describing the process of data analysis (e.g. sentiment analysis, word frequency count, etc.)</rdfs:comment>
        <rdfs:label xml:lang="en">Data Analysis</rdfs:label>
    </owl:Class>
    


    <!-- http://w3id.org/abdn/policy/pope#DataCollection -->

    <owl:Class rdf:about="http://w3id.org/abdn/policy/pope#DataCollection">
        <rdfs:subClassOf rdf:resource="http://w3id.org/abdn/policy/pope#ActivityPlan"/>
        <rdfs:comment xml:lang="en">A kind of  activity plan describing the process of data gathering (e.g. manual collection, collection using an API etc.)</rdfs:comment>
        <rdfs:label xml:lang="en">Data Collection</rdfs:label>
    </owl:Class>
    


    <!-- http://w3id.org/abdn/policy/pope#DataPreprocessing -->

    <owl:Class rdf:about="http://w3id.org/abdn/policy/pope#DataPreprocessing">
        <rdfs:subClassOf rdf:resource="http://w3id.org/abdn/policy/pope#ActivityPlan"/>
        <rdfs:comment xml:lang="en">A kind of activity plan describing the process of data preprocessing (e.g. stop words removal, filtering, text case transformation, etc.)</rdfs:comment>
        <rdfs:label xml:lang="en">Data Preprocessing</rdfs:label>
    </owl:Class>
    


    <!-- http://w3id.org/abdn/policy/pope#DataSet -->

    <owl:Class rdf:about="http://w3id.org/abdn/policy/pope#DataSet">
        <rdfs:subClassOf rdf:resource="http://www.w3.org/ns/prov#Role"/>
        <rdfs:comment xml:lang="en">A kind of role describing that the associated prov:Entity denoted a prov:Collection representing some dataset - i.e. a collection of dataset items.</rdfs:comment>
        <rdfs:label xml:lang="en">Data Set</rdfs:label>
    </owl:Class>
    


    <!-- http://w3id.org/abdn/policy/pope#LeafNode -->

    <owl:Class rdf:about="http://w3id.org/abdn/policy/pope#LeafNode">
        <rdfs:subClassOf rdf:resource="http://www.w3.org/2004/02/skos/core#Concept"/>
        <owl:disjointWith rdf:resource="http://w3id.org/abdn/policy/pope#OR_Node"/>
        <owl:disjointWith rdf:resource="http://w3id.org/abdn/policy/pope#XOR_Node"/>
        <rdfs:comment xml:lang="en">A concept describing a leaf node of a binary tree structure. The node is used to bind a 
a binary tree description of pope:Constraint to a specific pope:Parameter wich captures an aspect of the state of the world via subproperties of skos:related defined in PoPE. For eample, a parameter representing a keyword being included in a piece of text.</rdfs:comment>
        <rdfs:label xml:lang="en">Leaf Node</rdfs:label>
    </owl:Class>
    


    <!-- http://w3id.org/abdn/policy/pope#OR_Node -->

    <owl:Class rdf:about="http://w3id.org/abdn/policy/pope#OR_Node">
        <rdfs:subClassOf rdf:resource="http://www.w3.org/2004/02/skos/core#Concept"/>
        <owl:disjointWith rdf:resource="http://w3id.org/abdn/policy/pope#XOR_Node"/>
        <rdfs:comment xml:lang="en">A concept describing an inner node of a binary tree structure. The node represents the logical operator OR  in a binary tree description of pope:Constraint. If A is an OR_Node and B and C are children of A then  test on conditions specified by B OR C equals true.</rdfs:comment>
        <rdfs:label xml:lang="en">OR Node</rdfs:label>
    </owl:Class>
    


    <!-- http://w3id.org/abdn/policy/pope#Parameter -->

    <owl:Class rdf:about="http://w3id.org/abdn/policy/pope#Parameter">
        <rdfs:subClassOf rdf:resource="http://www.w3.org/ns/prov#Role"/>
        <rdfs:comment xml:lang="en">A kind of role describing that the associated prov:Entity denoted an activity parameter containing some information used in some data processing activity.</rdfs:comment>
        <rdfs:label xml:lang="en">Parameter</rdfs:label>
    </owl:Class>
    


    <!-- http://w3id.org/abdn/policy/pope#SentimentAnalysis -->

    <owl:Class rdf:about="http://w3id.org/abdn/policy/pope#SentimentAnalysis">
        <rdfs:subClassOf rdf:resource="http://w3id.org/abdn/policy/pope#DataAnalysis"/>
        <rdfs:comment xml:lang="en">A kind of activity plan describing analysis that utilises an algorithm to determine the sentiment (e.g. positive, negative, neutral) in a corpus of documents.</rdfs:comment>
        <rdfs:label xml:lang="en">Sentiment Analysis</rdfs:label>
    </owl:Class>
    


    <!-- http://w3id.org/abdn/policy/pope#TopicExtraction -->

    <owl:Class rdf:about="http://w3id.org/abdn/policy/pope#TopicExtraction">
        <rdfs:subClassOf rdf:resource="http://w3id.org/abdn/policy/pope#DataAnalysis"/>
        <rdfs:comment xml:lang="en">A kind activity plan describing  analysis that utilise and algorithm for extracting topics from a corpus of documents.</rdfs:comment>
        <rdfs:label xml:lang="en">Topic Extraction</rdfs:label>
    </owl:Class>
    


    <!-- http://w3id.org/abdn/policy/pope#XOR_Node -->

    <owl:Class rdf:about="http://w3id.org/abdn/policy/pope#XOR_Node">
        <rdfs:subClassOf rdf:resource="http://www.w3.org/2004/02/skos/core#Concept"/>
        <rdfs:comment xml:lang="en">A concept describing an inner node of a binary tree structure. The node represents the logical operator XOR in a binary tree description of pope:Constraint. If A is an XOR_Node and B and C are children of A then test on conditions specified by B XOR C equals true.</rdfs:comment>
        <rdfs:label xml:lang="en">XOR Node</rdfs:label>
    </owl:Class>
    


    <!-- 
    ///////////////////////////////////////////////////////////////////////////////////////
    //
    // Individuals
    //
    ///////////////////////////////////////////////////////////////////////////////////////
     -->

    


    <!-- http://w3id.org/abdn/policy/pope#ApiEndpoint -->

    <owl:NamedIndividual rdf:about="http://w3id.org/abdn/policy/pope#ApiEndpoint">
        <rdf:type rdf:resource="http://w3id.org/abdn/policy/pope#Parameter"/>
        <rdfs:comment xml:lang="en">A role describing that the associated prov:Entity denoted an activity parameter containing some information about an API reference endpoint used in some data processing activity.</rdfs:comment>
        <rdfs:label xml:lang="en">API Endpoint</rdfs:label>
    </owl:NamedIndividual>
    


    <!-- http://w3id.org/abdn/policy/pope#CollectionViaApi -->

    <owl:NamedIndividual rdf:about="http://w3id.org/abdn/policy/pope#CollectionViaApi">
        <rdf:type rdf:resource="http://w3id.org/abdn/policy/pope#ActivityPlan"/>
        <rdf:type rdf:resource="http://w3id.org/abdn/policy/pope#DataCollection"/>
        <rdfs:comment xml:lang="en">Collection of data retrieved via an API.</rdfs:comment>
        <rdfs:label xml:lang="en">Collection via API</rdfs:label>
    </owl:NamedIndividual>
    


    <!-- http://w3id.org/abdn/policy/pope#DataAddition -->

    <owl:NamedIndividual rdf:about="http://w3id.org/abdn/policy/pope#DataAddition">
        <rdf:type rdf:resource="http://w3id.org/abdn/policy/pope#ActivityPlan"/>
        <rdf:type rdf:resource="http://w3id.org/abdn/policy/pope#DataPreprocessing"/>
        <rdfs:comment xml:lang="en">Addition of data based on some parameters. Resulting dataset collection(s) will contain the same amount of data items as the sum of data items in collections used by the activity.</rdfs:comment>
        <rdfs:label xml:lang="en">Data Addition</rdfs:label>
    </owl:NamedIndividual>
    


    <!-- http://w3id.org/abdn/policy/pope#DataFiltering -->

    <owl:NamedIndividual rdf:about="http://w3id.org/abdn/policy/pope#DataFiltering">
        <rdf:type rdf:resource="http://w3id.org/abdn/policy/pope#ActivityPlan"/>
        <rdf:type rdf:resource="http://w3id.org/abdn/policy/pope#DataPreprocessing"/>
        <rdfs:comment xml:lang="en">Filtering of data based on some parameters. Resulting dataset collection(s) will contain only those data items that met the filtering conditions.</rdfs:comment>
        <rdfs:label xml:lang="en">Data Filtering</rdfs:label>
    </owl:NamedIndividual>
    <owl:Axiom>
        <owl:annotatedSource rdf:resource="http://w3id.org/abdn/policy/pope#DataFiltering"/>
        <owl:annotatedProperty rdf:resource="http://www.w3.org/1999/02/22-rdf-syntax-ns#type"/>
        <owl:annotatedTarget rdf:resource="http://w3id.org/abdn/policy/pope#DataPreprocessing"/>
        <rdfs:comment xml:lang="en">A kind of activity plan describing some data filtering process. The kind of filtering action is further described by prov:Entities used by the activity and described using pope:Parameter role, and associated PoPE subproperties of skos:related such as pope:includedIn, pope:subsumes, etc.   For example, and entity with the role pope:Keyword linked to the entities generated by the filtering activity via pope:includedIn denotes that the generated entities contain a specific keyword (subject to further constriants imposed on the parameters described using pope:Constraint).</rdfs:comment>
        <rdfs:label xml:lang="en">Filtering Process</rdfs:label>
    </owl:Axiom>
    


    <!-- http://w3id.org/abdn/policy/pope#DataRemoval -->

    <owl:NamedIndividual rdf:about="http://w3id.org/abdn/policy/pope#DataRemoval">
        <rdf:type rdf:resource="http://w3id.org/abdn/policy/pope#ActivityPlan"/>
        <rdf:type rdf:resource="http://w3id.org/abdn/policy/pope#DataPreprocessing"/>
        <rdfs:comment xml:lang="en">Removal of data s based on some parameters. Resulting dataset collection(s) will contain the same amount of data items as the sum of data items in collections used by the activity.</rdfs:comment>
        <rdfs:label xml:lang="en">Data Removal</rdfs:label>
    </owl:NamedIndividual>
    <owl:Axiom>
        <owl:annotatedSource rdf:resource="http://w3id.org/abdn/policy/pope#DataRemoval"/>
        <owl:annotatedProperty rdf:resource="http://www.w3.org/1999/02/22-rdf-syntax-ns#type"/>
        <owl:annotatedTarget rdf:resource="http://w3id.org/abdn/policy/pope#DataPreprocessing"/>
        <rdfs:comment xml:lang="en">A kind of activity plan describing some data removal process (e.g. a stop word removal). The kind of action is further described by prov:Entities used by the activity and described using pope:Parameter role, and associated PoPE subproperties of skos:related such as pope:includedIn, pope:subsumes, etc.  For example, and entity with role pope:Keyword linked to the entities generated by the filtering activity via pope:notIncludedIn denotes that the generated entities do not contain a specific keyword (subject to further constriants imposed on the parameters described using pope:Constraint).</rdfs:comment>
        <rdfs:label xml:lang="en">Data Removal</rdfs:label>
    </owl:Axiom>
    


    <!-- http://w3id.org/abdn/policy/pope#GroupTag -->

    <owl:NamedIndividual rdf:about="http://w3id.org/abdn/policy/pope#GroupTag">
        <rdf:type rdf:resource="http://w3id.org/abdn/policy/pope#Parameter"/>
        <rdfs:comment xml:lang="en">A role describing that the associated prov:Entity denoted an activity parameter containing some information about a group tag (e.g. to group multiple search activities) used in some data processing activity.</rdfs:comment>
        <rdfs:label xml:lang="en">Group Tag</rdfs:label>
    </owl:NamedIndividual>
    


    <!-- http://w3id.org/abdn/policy/pope#Keyword -->

    <owl:NamedIndividual rdf:about="http://w3id.org/abdn/policy/pope#Keyword">
        <rdf:type rdf:resource="http://w3id.org/abdn/policy/pope#Parameter"/>
        <rdfs:comment xml:lang="en">A role describing that the associated prov:Entity denoted an activity parameter containing some information about a keyword used in some data processing activity.</rdfs:comment>
        <rdfs:label xml:lang="en">Keyword</rdfs:label>
    </owl:NamedIndividual>
    


    <!-- http://w3id.org/abdn/policy/pope#LDA_TopicExtraction -->

    <owl:NamedIndividual rdf:about="http://w3id.org/abdn/policy/pope#LDA_TopicExtraction">
        <rdf:type rdf:resource="http://w3id.org/abdn/policy/pope#ActivityPlan"/>
        <rdf:type rdf:resource="http://w3id.org/abdn/policy/pope#DataAnalysis"/>
        <rdf:type rdf:resource="http://w3id.org/abdn/policy/pope#TopicExtraction"/>
        <rdfs:comment xml:lang="en">A topic extraction utilising the LDA algorithm.</rdfs:comment>
        <rdfs:label xml:lang="en">Latent Dirichlet Allocation Topic Exctraction</rdfs:label>
    </owl:NamedIndividual>
    


    <!-- http://w3id.org/abdn/policy/pope#Location -->

    <owl:NamedIndividual rdf:about="http://w3id.org/abdn/policy/pope#Location">
        <rdf:type rdf:resource="http://w3id.org/abdn/policy/pope#Parameter"/>
        <rdfs:comment xml:lang="en">A role describing that the associated prov:Entity denoted an activity parameter containing some information about a location used in some data processing activity.</rdfs:comment>
        <rdfs:label xml:lang="en">Location</rdfs:label>
    </owl:NamedIndividual>
    


    <!-- http://w3id.org/abdn/policy/pope#MultiLayerPerceptronNeuralNetworksSentimentAnalysis -->

    <owl:NamedIndividual rdf:about="http://w3id.org/abdn/policy/pope#MultiLayerPerceptronNeuralNetworksSentimentAnalysis">
        <rdf:type rdf:resource="http://w3id.org/abdn/policy/pope#ActivityPlan"/>
        <rdf:type rdf:resource="http://w3id.org/abdn/policy/pope#DataAnalysis"/>
        <rdf:type rdf:resource="http://w3id.org/abdn/policy/pope#SentimentAnalysis"/>
        <rdfs:comment xml:lang="en">A sentiment analysis utilising the Multi-Layer Perceptron Neural Networks algorithm.</rdfs:comment>
        <rdfs:label xml:lang="en">Multi-Layer Perceptron Neural Networks Sentiment Analysis</rdfs:label>
    </owl:NamedIndividual>
    


    <!-- http://w3id.org/abdn/policy/pope#NaiveBayesSentimentAnalysis -->

    <owl:NamedIndividual rdf:about="http://w3id.org/abdn/policy/pope#NaiveBayesSentimentAnalysis">
        <rdf:type rdf:resource="http://w3id.org/abdn/policy/pope#ActivityPlan"/>
        <rdf:type rdf:resource="http://w3id.org/abdn/policy/pope#DataAnalysis"/>
        <rdf:type rdf:resource="http://w3id.org/abdn/policy/pope#SentimentAnalysis"/>
        <rdfs:comment xml:lang="en">A sentiment analysis utilising the naïve Bayes algorithm.</rdfs:comment>
        <rdfs:label xml:lang="en">Naïve Bayes Sentiment Analysis</rdfs:label>
    </owl:NamedIndividual>
    


    <!-- http://w3id.org/abdn/policy/pope#NewsArticleDataSet -->

    <owl:NamedIndividual rdf:about="http://w3id.org/abdn/policy/pope#NewsArticleDataSet">
        <rdf:type rdf:resource="http://w3id.org/abdn/policy/pope#DataSet"/>
        <rdfs:comment xml:lang="en">A kind of role describing that the associated prov:Entity denoted a prov:Collection representing a collection of news articles.</rdfs:comment>
        <rdfs:label xml:lang="en">News Article Dataset</rdfs:label>
    </owl:NamedIndividual>
    


    <!-- http://w3id.org/abdn/policy/pope#PopeSkosSchema -->

    <owl:NamedIndividual rdf:about="http://w3id.org/abdn/policy/pope#PopeSkosSchema">
        <rdf:type rdf:resource="http://www.w3.org/2004/02/skos/core#ConceptScheme"/>
        <rdfs:comment xml:lang="en">PoPE skos schemea. Skos concepts defined using PoPE should be linked to this schema via skos:inSchema.</rdfs:comment>
        <rdfs:label xml:lang="en">PoPE Skos Schema</rdfs:label>
    </owl:NamedIndividual>
    


    <!-- http://w3id.org/abdn/policy/pope#PostID -->

    <owl:NamedIndividual rdf:about="http://w3id.org/abdn/policy/pope#PostID">
        <rdf:type rdf:resource="http://w3id.org/abdn/policy/pope#Parameter"/>
        <rdfs:comment xml:lang="en">A role describing that the associated prov:Entity denoted an activity parameter containing some information about an ID of a social media post used in some data processing activity.</rdfs:comment>
        <rdfs:label xml:lang="en">Post ID</rdfs:label>
    </owl:NamedIndividual>
    


    <!-- http://w3id.org/abdn/policy/pope#Postcondition -->

    <owl:NamedIndividual rdf:about="http://w3id.org/abdn/policy/pope#Postcondition">
        <rdf:type rdf:resource="http://w3id.org/abdn/policy/pope#Constraint"/>
        <rdfs:comment xml:lang="en">A kind of role describing that the associated prov:Entity denoted a poscondition constraint used by some activity describing a state of the world that entities generated this activity conformed to.</rdfs:comment>
        <rdfs:label xml:lang="en">Postcondition</rdfs:label>
    </owl:NamedIndividual>
    <owl:Axiom>
        <owl:annotatedSource rdf:resource="http://w3id.org/abdn/policy/pope#Postcondition"/>
        <owl:annotatedProperty rdf:resource="http://www.w3.org/1999/02/22-rdf-syntax-ns#type"/>
        <owl:annotatedTarget rdf:resource="http://w3id.org/abdn/policy/pope#Constraint"/>
        <rdfs:comment xml:lang="en">An activity postcondition describes a state of the world that generated entities conformed to. The state is described as logical groupings of one or more pope:Parameter use dby the activity and semantically linked with subproperties of skos:related to some characterists of generated datasets or dataset items.</rdfs:comment>
        <rdfs:label xml:lang="en">Postcondition</rdfs:label>
    </owl:Axiom>
    


    <!-- http://w3id.org/abdn/policy/pope#Precondition -->

    <owl:NamedIndividual rdf:about="http://w3id.org/abdn/policy/pope#Precondition">
        <rdf:type rdf:resource="http://w3id.org/abdn/policy/pope#Constraint"/>
        <rdfs:comment xml:lang="en">A kind of role describing that the associated prov:Entity denoted a poscondition constraint used by some activity describing a state of the world that entities conformed to before this activity ended. For example, a precondition can be described with a parameter denoting a threshold for the  maximum number of data items that can be processed by an activity.</rdfs:comment>
        <rdfs:label xml:lang="en">Precondition</rdfs:label>
    </owl:NamedIndividual>
    <owl:Axiom>
        <owl:annotatedSource rdf:resource="http://w3id.org/abdn/policy/pope#Precondition"/>
        <owl:annotatedProperty rdf:resource="http://www.w3.org/1999/02/22-rdf-syntax-ns#type"/>
        <owl:annotatedTarget rdf:resource="http://w3id.org/abdn/policy/pope#Constraint"/>
        <rdfs:comment xml:lang="en">An activity precondition describes a state of the world that used entities conformed to. The state is described as logical groupings of one or more pope:Parameter used by the activity and semantically linked with subproperties of skos:related to some characterists of used datasets or dataset items.</rdfs:comment>
        <rdfs:label xml:lang="en">Precondition</rdfs:label>
    </owl:Axiom>
    


    <!-- http://w3id.org/abdn/policy/pope#Regex -->

    <owl:NamedIndividual rdf:about="http://w3id.org/abdn/policy/pope#Regex">
        <rdf:type rdf:resource="http://w3id.org/abdn/policy/pope#Parameter"/>
        <rdfs:comment xml:lang="en">A role describing that the associated prov:Entity denoted an activity parameter containing some information about a regular expression used in some data processing activity.</rdfs:comment>
        <rdfs:comment xml:lang="en">Regex</rdfs:comment>
    </owl:NamedIndividual>
    


    <!-- http://w3id.org/abdn/policy/pope#SentimentAnalysisDataSet -->

    <owl:NamedIndividual rdf:about="http://w3id.org/abdn/policy/pope#SentimentAnalysisDataSet">
        <rdf:type rdf:resource="http://w3id.org/abdn/policy/pope#DataSet"/>
        <rdfs:comment xml:lang="en">A kind of role describing that the associated prov:Entity denoted a prov:Collection representing  sentiment analysis results collection.</rdfs:comment>
        <rdfs:label xml:lang="en">Sentiment Analysis Dataset</rdfs:label>
    </owl:NamedIndividual>
    


    <!-- http://w3id.org/abdn/policy/pope#StatisticalMeasure -->

    <owl:NamedIndividual rdf:about="http://w3id.org/abdn/policy/pope#StatisticalMeasure">
        <rdf:type rdf:resource="http://w3id.org/abdn/policy/pope#Parameter"/>
        <rdfs:comment xml:lang="en">A role describing that the associated prov:Entity denoted an activity parameter containing some information about a statistical measure (e.g.  dataset size) used in some data processing activity.</rdfs:comment>
        <rdfs:label xml:lang="en">Statistical Measure</rdfs:label>
    </owl:NamedIndividual>
    


    <!-- http://w3id.org/abdn/policy/pope#TextObject -->

    <owl:NamedIndividual rdf:about="http://w3id.org/abdn/policy/pope#TextObject">
        <rdf:type rdf:resource="http://w3id.org/abdn/policy/pope#Parameter"/>
        <rdfs:comment xml:lang="en">A role describing that the associated prov:Entity denoted an activity parameter containing some information about a piece of text used in some data processing activity.</rdfs:comment>
        <rdfs:label xml:lang="en">Text Object</rdfs:label>
    </owl:NamedIndividual>
    


    <!-- http://w3id.org/abdn/policy/pope#TextToLowerCase -->

    <owl:NamedIndividual rdf:about="http://w3id.org/abdn/policy/pope#TextToLowerCase">
        <rdf:type rdf:resource="http://w3id.org/abdn/policy/pope#ActivityPlan"/>
        <rdf:type rdf:resource="http://w3id.org/abdn/policy/pope#DataPreprocessing"/>
        <rdfs:comment xml:lang="en">Conversion of text to lowercase.</rdfs:comment>
        <rdfs:label xml:lang="en">Text To Lower Case</rdfs:label>
    </owl:NamedIndividual>
    <owl:Axiom>
        <owl:annotatedSource rdf:resource="http://w3id.org/abdn/policy/pope#TextToLowerCase"/>
        <owl:annotatedProperty rdf:resource="http://www.w3.org/1999/02/22-rdf-syntax-ns#type"/>
        <owl:annotatedTarget rdf:resource="http://w3id.org/abdn/policy/pope#DataPreprocessing"/>
        <rdfs:comment xml:lang="en">A kind of activity plan describing a process converting text to lowercase. This kind of action is further described by prov:Entities used by the activity and described using pope:Parameter role, and associated PoPE subproperties of skos:related such as pope:includedIn, pope:subsumes, etc.   For example, and entity with role pope:Regex representing uppercase letters linked to some characteristics of entities (data items) generated by the activity via pope:doesNotMatch denotes that the generated entities contain a text that does not contain any uppercase letters (subject to further constriants imposed on the parameters described using pope:Constraint).</rdfs:comment>
        <rdfs:label xml:lang="en">Text to lowercase</rdfs:label>
    </owl:Axiom>
    


    <!-- http://w3id.org/abdn/policy/pope#TextToUpperCase -->

    <owl:NamedIndividual rdf:about="http://w3id.org/abdn/policy/pope#TextToUpperCase">
        <rdf:type rdf:resource="http://w3id.org/abdn/policy/pope#ActivityPlan"/>
        <rdf:type rdf:resource="http://w3id.org/abdn/policy/pope#DataPreprocessing"/>
        <rdfs:comment xml:lang="en">Conversion of text to uppercase.</rdfs:comment>
        <rdfs:label xml:lang="en">Text To Upper Case</rdfs:label>
    </owl:NamedIndividual>
    <owl:Axiom>
        <owl:annotatedSource rdf:resource="http://w3id.org/abdn/policy/pope#TextToUpperCase"/>
        <owl:annotatedProperty rdf:resource="http://www.w3.org/1999/02/22-rdf-syntax-ns#type"/>
        <owl:annotatedTarget rdf:resource="http://w3id.org/abdn/policy/pope#DataPreprocessing"/>
        <rdfs:comment xml:lang="en">A kind of activity plan describing a process converting text to uppercase. This kind of action is further described by prov:Entities used by the activity and described using pope:Parameter role, and associated PoPE subproperties of skos:related such as pope:includedIn, pope:subsumes, etc.   For example, and entity with role pope:Regex representing lowercase letters linked to some characteristics of entities (data items) generated by the activity via pope:doesNotMatch denotes that the generated entities contain a text that does not contain any lowercase letters (subject to further constriants imposed on the parameters described using pope:Constraint).</rdfs:comment>
        <rdfs:label xml:lang="en">Text to uppercase</rdfs:label>
    </owl:Axiom>
    


    <!-- http://w3id.org/abdn/policy/pope#Time -->

    <owl:NamedIndividual rdf:about="http://w3id.org/abdn/policy/pope#Time">
        <rdf:type rdf:resource="http://w3id.org/abdn/policy/pope#Parameter"/>
        <rdfs:comment xml:lang="en">A role describing that the associated prov:Entity denoted an activity parameter containing some information about time used in some data processing activity.</rdfs:comment>
        <rdfs:label xml:lang="en">Time</rdfs:label>
    </owl:NamedIndividual>
    


    <!-- http://w3id.org/abdn/policy/pope#TopicExtractionDataSet -->

    <owl:NamedIndividual rdf:about="http://w3id.org/abdn/policy/pope#TopicExtractionDataSet">
        <rdf:type rdf:resource="http://w3id.org/abdn/policy/pope#DataSet"/>
        <rdfs:comment xml:lang="en">A kind of role describing that the associated prov:Entity denoted a prov:Collection representing topic extraction results collection.</rdfs:comment>
        <rdfs:label xml:lang="en">Topic Extraction Dataset</rdfs:label>
    </owl:NamedIndividual>
    


    <!-- http://w3id.org/abdn/policy/pope#TwitterDataset -->

    <owl:NamedIndividual rdf:about="http://w3id.org/abdn/policy/pope#TwitterDataset">
        <rdf:type rdf:resource="http://w3id.org/abdn/policy/pope#DataSet"/>
        <rdfs:comment xml:lang="en">A kind of role describing that the associated prov:Entity denoted a prov:Collection representing a collection of posts from Twitter social media platform.</rdfs:comment>
        <rdfs:label xml:lang="en">Twitter Dataset</rdfs:label>
    </owl:NamedIndividual>
    


    <!-- http://w3id.org/abdn/policy/pope#WordFrequencyCount -->

    <owl:NamedIndividual rdf:about="http://w3id.org/abdn/policy/pope#WordFrequencyCount">
        <rdf:type rdf:resource="http://w3id.org/abdn/policy/pope#ActivityPlan"/>
        <rdf:type rdf:resource="http://w3id.org/abdn/policy/pope#DataAnalysis"/>
        <rdfs:comment xml:lang="en">Analysis of single word frequency in a piece of text. Can be restricted by parameters specifying the number of top frequent words returned.</rdfs:comment>
        <rdfs:label xml:lang="en">Word Frequency Count</rdfs:label>
    </owl:NamedIndividual>
    


    <!-- http://w3id.org/abdn/policy/pope#WordFrequencyDataSet -->

    <owl:NamedIndividual rdf:about="http://w3id.org/abdn/policy/pope#WordFrequencyDataSet">
        <rdf:type rdf:resource="http://w3id.org/abdn/policy/pope#DataSet"/>
        <rdfs:comment xml:lang="en">A kind of role describing that the associated prov:Entity denoted a prov:Collection representing  word frequency  results collection.</rdfs:comment>
        <rdfs:label xml:lang="en">Word Frequency Dataset</rdfs:label>
    </owl:NamedIndividual>
</rdf:RDF>



<!-- Generated by the OWL API (version 4.2.5.20160517-0735) https://github.com/owlcs/owlapi -->

